library/init/category/state.lean
@@ -2,6 +2,8 @@
 Copyright (c) 2016 Microsoft Corporation. All rights reserved.
 Released under Apache 2.0 license as described in the file LICENSE.
 Authors: Leonardo de Moura, Sebastian Ullrich
+
+The state monad transformer.
 -/
 prelude
 import init.category.alternative init.category.lift
@@ -17,60 +19,62 @@ attribute [pp_using_anonymous_constructor] state_t
 
 namespace state_t
 section
-  variable  {σ : Type u}
-  variable  {m : Type u → Type v}
+  variables {σ : Type u} {m : Type u → Type v}
 
+  -- swap `st` and `x`
   @[inline] protected def run {α : Type u} (st : σ) (x : state_t σ m α) : m (α × σ) :=
   state_t.run' x st
 
   variable  [monad m]
   variables {α β : Type u}
 
-  protected def pure (a : α) : state_t σ m α :=
+  @[inline] protected def pure (a : α) : state_t σ m α :=
   ⟨λ s, pure (a, s)⟩
 
-  protected def bind (act₁ : state_t σ m α) (act₂ : α → state_t σ m β) : state_t σ m β :=
-  ⟨λ s, do (a, new_s) ← act₁.run s,
-           (act₂ a).run new_s⟩
+  @[inline] protected def bind (x : state_t σ m α) (f : α → state_t σ m β) : state_t σ m β :=
+  ⟨λ s, do (a, s') ← x.run s,
+           (f a).run s'⟩
 
   instance : monad (state_t σ m) :=
-  { pure := @state_t.pure σ m _, bind := @state_t.bind σ m _ }
+  { pure := @state_t.pure _ _ _, bind := @state_t.bind _ _ _ }
 
-  protected def orelse [alternative m] (α : Type u) (act₁ act₂ : state_t σ m α) : state_t σ m α :=
-  ⟨λ s, act₁.run s <|> act₂.run s⟩
+  protected def orelse [alternative m] {α : Type u} (x₁ x₂ : state_t σ m α) : state_t σ m α :=
+  ⟨λ s, x₁.run s <|> x₂.run s⟩
 
-  protected def failure [alternative m] (α : Type u) : state_t σ m α :=
+  protected def failure [alternative m] {α : Type u} : state_t σ m α :=
   ⟨λ s, failure⟩
 
   instance [alternative m] : alternative (state_t σ m) :=
-  { failure := @state_t.failure σ m _ _,
-    orelse  := @state_t.orelse σ m _ _,
-    ..state_t.monad }
+  { failure := @state_t.failure _ _ _ _,
+    orelse  := @state_t.orelse _ _ _ _ }
 
-  protected def get : state_t σ m σ :=
-  ⟨λ s, return (s, s)⟩
+  @[inline] protected def get : state_t σ m σ :=
+  ⟨λ s, pure (s, s)⟩
 
-  protected def put : σ → state_t σ m punit :=
-  λ s', ⟨λ s, return (punit.star, s')⟩
+  @[inline] protected def put : σ → state_t σ m punit :=
+  λ s', ⟨λ s, pure (punit.star, s')⟩
 
-  protected def modify (f : σ → σ) : state_t σ m punit :=
-  ⟨λ s, return (punit.star, f s)⟩
+  @[inline] protected def modify (f : σ → σ) : state_t σ m punit :=
+  ⟨λ s, pure (punit.star, f s)⟩
 
-  protected def lift {α : Type u} (t : m α) : state_t σ m α :=
-  ⟨λ s, do a ← t, return (a, s)⟩
+  @[inline] protected def lift {α : Type u} (t : m α) : state_t σ m α :=
+  ⟨λ s, do a ← t, pure (a, s)⟩
 
   instance : has_monad_lift m (state_t σ m) :=
   ⟨@state_t.lift σ m _⟩
 
-  protected def monad_map {σ m m'} [monad m] [monad m'] {α} (f : Π {α}, m α → m' α) : state_t σ m α → state_t σ m' α :=
+  @[inline] protected def monad_map {σ m m'} [monad m] [monad m'] {α} (f : Π {α}, m α → m' α) :
+    state_t σ m α → state_t σ m' α :=
   λ x, ⟨λ st, f (x.run st)⟩
 
   instance (σ m m') [monad m] [monad m'] : monad_functor m m' (state_t σ m) (state_t σ m') :=
   ⟨@state_t.monad_map σ m m' _ _⟩
 
   -- TODO(Sebastian): uses lenses as in https://hackage.haskell.org/package/lens-4.15.4/docs/Control-Lens-Zoom.html#t:Zoom ?
-  protected def zoom {σ σ' α : Type u} {m : Type u → Type v} [monad m] (get : σ → σ') (set : σ' → σ → σ) (x : state_t σ' m α) : state_t σ m α :=
-  ⟨λ st, (λ p : α × σ', (p.fst, set p.snd st)) <$> x.run (get st)⟩
+  protected def zoom {σ σ' α : Type u} {m : Type u → Type v} [monad m] (get : σ → σ')
+    (set : σ' → σ → σ) (x : state_t σ' m α) : state_t σ m α :=
+  ⟨λ st, do (a, st') ← x.run (get st),
+            pure (a, set st' st)⟩
 
   instance (ε) [monad_except ε m] : monad_except ε (state_t σ m) :=
   { throw := λ α, state_t.lift ∘ throw,
@@ -81,6 +85,8 @@ end state_t
 @[reducible] protected def state.run {σ α : Type u} (st : σ) (x : state σ α) : α × σ :=
 state_t.run st x
 
+
+/-- A specialization of `monad_lift` to `state_t` that allows `σ` to be inferred. -/
 class monad_state_lift (σ : out_param (Type u)) (m : out_param (Type u → Type v)) (n : Type u → Type w) :=
 [has_lift : has_monad_lift_t (state_t σ m) n]
 
@@ -103,13 +109,16 @@ monad_lift (state_t.put st : state_t σ m _)
 monad_lift (state_t.modify f : state_t σ m _)
 end
 
+
+/-- A specialization of `monad_map` to `state_t` that allows `σ` to be inferred. -/
 class monad_state_functor (σ σ' : out_param (Type u)) (m : out_param (Type u → Type v)) (n n' : Type u → Type w) :=
 [functor {} : monad_functor_t (state_t σ m) (state_t σ' m) n n']
 
 attribute [instance] monad_state_functor.mk
 local attribute [instance] monad_state_functor.functor
 
-def zoom {σ σ'} {m n n'} [monad m] {α : Type u} (get : σ → σ') (set : σ' → σ → σ) [monad_state_functor σ' σ m n n'] : n α → n' α :=
+def zoom {σ σ'} {m n n'} [monad m] {α : Type u} (get : σ → σ') (set : σ' → σ → σ)
+  [monad_state_functor σ' σ m n n'] : n α → n' α :=
 monad_map $ λ α, (state_t.zoom get set : state_t σ' m α → state_t σ m α)
 
 instance (σ m out) [monad_run out m] : monad_run (λ α, σ → out (α × σ)) (state_t σ m) :=
