library/init/category/id.lean
@@ -2,6 +2,8 @@
 Copyright (c) 2017 Microsoft Corporation. All rights reserved.
 Released under Apache 2.0 license as described in the file LICENSE.
 Authors: Sebastian Ullrich
+
+The identity monad.
 -/
 prelude
 import init.category.lift
