library/init/category/monad.lean
@@ -24,7 +24,7 @@ class monad (m : Type u → Type v) extends applicative m, has_bind m : Type (ma
 (map := λ α β f x, x >>= pure ∘ f)
 (seq := λ α β f x, f >>= (<$> x))
 
-@[reducible] def return {m : Type u → Type v} [monad m] {α : Type u} : α → m α :=
+@[reducible, inline] def return {m : Type u → Type v} [monad m] {α : Type u} : α → m α :=
 pure
 
 /- Identical to has_bind.and_then, but it is not inlined. -/
