library/init/category/monad_fail.lean
@@ -18,5 +18,5 @@ def match_failed {α : Type u} {m : Type u → Type v} [monad_fail m] : m α :=
 monad_fail.fail "match failed"
 
 -- TODO(Sebastian): Could take `has_monad_lift_t`, except that the refl instances will make it loop
-instance monad_fail_lift (m n : Type u → Type v) [has_monad_lift m n] [monad_fail m] [monad_n : monad n] : monad_fail n :=
-{ fail := λ α s, monad_lift (monad_fail.fail s : m α), ..monad_n }
+instance monad_fail_lift (m n : Type u → Type v) [has_monad_lift m n] [monad_fail m] [monad n] : monad_fail n :=
+{ fail := λ α s, monad_lift (monad_fail.fail s : m α) }
