library/init/category/reader.lean
@@ -2,6 +2,8 @@
 Copyright (c) 2017 Microsoft Corporation. All rights reserved.
 Released under Apache 2.0 license as described in the file LICENSE.
 Authors: Sebastian Ullrich
+
+The reader monad transformer for passing immutable state.
 -/
 
 prelude
@@ -12,6 +14,8 @@ structure reader_t (r : Type u) (m : Type u → Type v) (α : Type u) : Type (ma
 (run : r → m α)
 
 @[reducible] def reader (r : Type u) := reader_t r id
+
+attribute [pp_using_anonymous_constructor] reader_t
 
 namespace reader_t
 section
@@ -47,6 +51,8 @@ section
 end
 end reader_t
 
+
+/-- A specialization of `monad_lift` to `reader_t` that allows `r` to be inferred. -/
 class monad_reader_lift (r : out_param (Type u)) (m : out_param (Type u → Type v)) (n : Type u → Type w) :=
 [has_lift : has_monad_lift_t (reader_t r m) n]
 
@@ -57,6 +63,8 @@ def monad_reader_lift.read {r : Type u} {m : Type u → Type v} {n : Type u → 
 @monad_lift _ _ _ _ (reader_t.read : reader_t r m _)
 export monad_reader_lift (read)
 
+
+/-- A specialization of `monad_map` to `reader_t` that allows `r` to be inferred. -/
 class monad_reader_functor (r r' : out_param (Type u)) (m : out_param (Type u → Type v)) (n n' : Type u → Type w) :=
 [functor {} : monad_functor_t (reader_t r m) (reader_t r' m) n n']
 
@@ -68,6 +76,7 @@ def with_reader_t {r r' m} [monad m] {α} (f : r' → r) : reader_t r m α → r
 
 def with_reader {r r'} {m n n'} [monad m] [monad_reader_functor r r' m n n'] {α : Type u} (f : r' → r) : n α → n' α :=
 monad_map $ λ α, (with_reader_t f : reader_t r m α → reader_t r' m α)
+
 
 instance (r : Type u) (m out) [monad_run out m] : monad_run (λ α, r → out α) (reader_t r m) :=
 ⟨λ α x, run ∘ x.run, λ α a, reader_t.mk (unrun ∘ a)⟩
